equiv/AxiomCheck.lean
@@ -8,22 +8,10 @@ deliberately and update the pinned messages below. -/
 
 /-- info: 'SHS.Equiv.SHA256.sha256_correct' depends on axioms: [propext,
  Classical.choice,
- Quot.sound,
- SHS.Equiv.SHA256.Functions.Maj_toBitVec._native.bv_decide.ax_1_6,
- SHS.Equiv.SHA256.Functions.bigSigma0_toBitVec._native.bv_decide.ax_1_6,
- SHS.Equiv.SHA256.Functions.bigSigma1_toBitVec._native.bv_decide.ax_1_6,
- SHS.Equiv.SHA256.Functions.smallSigma0_toBitVec._native.bv_decide.ax_1_6,
- SHS.Equiv.SHA256.Functions.smallSigma1_toBitVec._native.bv_decide.ax_1_6,
- SHS.Equiv.SHA256.ToU32s.beU32_eq_fromBits._native.bv_decide.ax_1_5,
- SHS.Equiv.SHA256.Digest.fromBits_4bytes_BE_256._native.bv_decide.ax_1_9✝] -/
+ Lean.ofReduceBool,
+ Lean.trustCompiler,
+ Quot.sound] -/
 #guard_msgs in #print axioms SHS.Equiv.SHA256.sha256_correct
 
-/-- info: 'SHS.Equiv.SHA256.compress_correct' depends on axioms: [propext,
- Classical.choice,
- Quot.sound,
- SHS.Equiv.SHA256.Functions.Maj_toBitVec._native.bv_decide.ax_1_6,
- SHS.Equiv.SHA256.Functions.bigSigma0_toBitVec._native.bv_decide.ax_1_6,
- SHS.Equiv.SHA256.Functions.bigSigma1_toBitVec._native.bv_decide.ax_1_6,
- SHS.Equiv.SHA256.Functions.smallSigma0_toBitVec._native.bv_decide.ax_1_6,
- SHS.Equiv.SHA256.Functions.smallSigma1_toBitVec._native.bv_decide.ax_1_6] -/
+/-- info: 'SHS.Equiv.SHA256.compress_correct' depends on axioms: [propext, Classical.choice, Quot.sound] -/
 #guard_msgs in #print axioms SHS.Equiv.SHA256.compress_correct
