lakefile.lean
@@ -15,10 +15,10 @@ package «fips-pub-180-4» where
   ]
 
 require mdgen from git
-  "https://github.com/Seasawher/mdgen" @ "main"
+  "https://github.com/Seasawher/mdgen" @ "v4.28.0-rc1"
 
 require mathlib from git
-  "https://github.com/leanprover-community/mathlib4" @ "v4.30.0-rc1"
+  "https://github.com/leanprover-community/mathlib4" @ "v4.28.0-rc1"
 
 @[default_target]
 lean_lib spec where
